Trying to prove Steel.Pointer

ulib/Steel.Pointer.Views.fst
@@ -1,6 +1,6 @@
 module Steel.Pointer.Views
 
-module A = LowStar.Array
+module A = Steel.Array
 module HS = FStar.HyperStack
 module P = LowStar.Permissions
 
@@ -12,44 +12,25 @@ open Steel.RST
 let pointer (t: Type) = ptr:A.array t{A.vlength ptr = 1}
 
 noeq type vptr (a: Type) = {
-  x: a;
-  p: P.permission
+  ptr_x: a;
+  ptr_p: P.permission
 }
 
-abstract
-let ptr_view (#a:Type) (ptr:pointer a) : view (vptr a) =
-  reveal_view ();
-  let fp (h: HS.mem) = A.loc_array ptr in
-  let inv (h: HS.mem): prop = A.live h ptr /\ A.vlength ptr = 1 in
-  let sel h = {x = Seq.index (A.as_seq h ptr) 0; p = A.get_perm h ptr 0} in
-  {
-    fp = fp;
-    inv = inv;
-    sel = sel
-  }
 
 let ptr_resource (#a:Type) (ptr:pointer a) =
-  as_resource (ptr_view ptr)
-
-let reveal_ptr ()
-  : Lemma ((forall a (ptr:pointer a) h .{:pattern as_loc (fp (ptr_resource ptr)) h}
-             as_loc (fp (ptr_resource ptr)) h == A.loc_array ptr) /\
-           (forall a (ptr:pointer a) h .{:pattern inv (ptr_resource ptr) h}
-             inv (ptr_resource ptr) h <==> A.live h ptr /\ A.vlength ptr = 1) /\
-           (forall a (ptr:pointer a) h .{:pattern sel (ptr_view ptr) h}
-             sel (ptr_view ptr) h == { x = Seq.index (A.as_seq h ptr) 0; p = A.get_perm h ptr 0})) =
-  ()
+  refine_view (A.array_resource ptr) (fun av -> { ptr_x = Seq.index av.A.s 0; ptr_p = av.A.p })
 
 let get_val
   (#a: Type)
   (ptr: pointer a)
   (#r: resource{ptr_resource #a ptr `is_subresource_of` r})
   (h: rmem r) : GTot a =
-  (h (ptr_resource ptr)).x
+  (h (ptr_resource ptr)).ptr_x
 
 let get_perm
   (#a: Type)
   (ptr: pointer a)
   (#r: resource{ptr_resource #a ptr `is_subresource_of` r})
   (h: rmem r) : GTot P.permission =
-  (h (ptr_resource ptr)).p
+  let v : vptr a = h (ptr_resource ptr) in
+  v.ptr_p
